Inclusion of permissions. In order to make type inclusion working, I had to change the inclusion of types also.

perm.v
@@ -1,4 +1,5 @@
 From iris.program_logic Require Import thread_local.
+From iris.proofmode Require Import invariants.
 From lrust Require Export type.
 
 Delimit Scope perm_scope with P.
@@ -8,9 +9,10 @@ Module Perm.
 
 Section perm.
 
-  Context `{lifetimeG Σ}.
+  Context `{heapG Σ, lifetimeG Σ, thread_localG Σ}.
 
-  (* TODO : define valuable expressions ν in order to define ν ◁ τ. *)
+  Definition has_type (v : val) (ty : type) : perm :=
+    λ tid, ty.(ty_own) tid [v].
 
   Definition extract (κ : lifetime) (ρ : perm) : perm :=
     λ tid, (κ ∋ ρ tid)%I.
@@ -27,7 +29,7 @@ Section perm.
   Definition sep (ρ1 ρ2 : perm) : @perm Σ :=
     λ tid, (ρ1 tid ★ ρ2 tid)%I.
 
-  Definition top : @perm Σ :=
+  Global Instance top : Top (@perm Σ) :=
     λ _, True%I.
 
 End perm.
@@ -35,6 +37,9 @@ End perm.
 End Perm.
 
 Import Perm.
+
+Notation "v ◁ ty" := (has_type v ty)
+  (at level 75, right associativity) : perm_scope.
 
 Notation "κ ∋ ρ" := (extract κ ρ)
   (at level 75, right associativity) : perm_scope.
@@ -47,8 +52,3 @@ Notation "∃ x .. y , P" :=
   (exist (λ x, .. (exist (λ y, P)) ..)) : perm_scope.
 
 Infix "★" := sep (at level 80, right associativity) : perm_scope.
-
-Notation "⊤" := top : perm_scope.
-
-Definition perm_incl {Σ} (ρ1 ρ2 : @perm Σ) :=
-  ∀ tid, ρ1 tid ⊢ ρ2 tid.
